slr-parsing/parserTermDefScript.sml
@@ -1,12 +1,16 @@
-open HolKernel boolLib bossLib Parse BasicProvers Defn
+open HolKernel boolLib bossLib Parse BasicProvers Defn;
 
 open listTheory containerTheory pred_setTheory arithmeticTheory
-relationTheory markerTheory boolSimps optionTheory
+     relationTheory markerTheory boolSimps optionTheory;
 
 open symbolDefTheory grammarDefTheory boolLemmasTheory listLemmasTheory
-parseTreeTheory parserDefTheory yaccDefTheory 
+     parseTreeTheory (* parserDefTheory *) yaccDefTheory ;
 
+val _ = new_theory "parserTermDef";
 
+(* Empty theory .... does this do something useful? *)
+
+val _ = export_theory();
 
 
 
